@prefix rdf:    <http://www.w3.org/1999/02/22-rdf-syntax-ns#> .
@prefix rdfs:   <http://www.w3.org/2000/01/rdf-schema#> .
@prefix sc:     <https://w3di.org/idlab/ns/supply-chain/#> .
@prefix schema: <https://schema.org/> .
@prefix xsd:    <http://www.w3.org/2001/XMLSchema#> .
@prefix dct:    <http://purl.org/dc/terms/> .
@prefix foaf:   <http://xmlns.com/foaf/0.1/>.

sc:
    rdfs:comment """Supply chain vocabulary""" ;
    dct:title    "Supply chain vocabulary"@en ;
    dct:issued   "2021-09-21"^^xsd:date ;
    dct:modified "2021-10-27"^^xsd:date ;
    dct:creator  [ foaf:mbox "pieter.heyvaert@ugent.be" ;
                   foaf:name "Pieter Heyvaert" ] .

# Classes

sc:LocationToLocation
    a               rdfs:Class ;
    rdfs:subClassOf schema:Thing ;
    rdfs:label      "Location to Location" ;
    rdfs:comment    "This represents information about transporting items from one location to another." .

sc:SupplierItemLocationOption
    a               rdfs:Class ;
    rdfs:subClassOf schema:Thing ;
    rdfs:label      "Supplier Item Location Option" ;
    rdfs:comment    "This represents a combination of a supplier and an item at a specification location." .

sc:LocationItemOption
    a               rdfs:Class ;
    rdfs:subClassOf schema:Thing ;
    rdfs:label      "Location Item Option" ;
    rdfs:comment    "This represents a combination of a location and an item." .

sc:SupplierItemLeadTimeOption
    a               rdfs:Class ;
    rdfs:subClassOf schema:Thing ;
    rdfs:label      "Supplier Item LeadTime Option" ;
    rdfs:comment    "This represents a combination of a supplier, an item and a lead time." .

sc:CustomerItemOption
    a               rdfs:Class ;
    rdfs:subClassOf schema:Thing ;
    rdfs:label      "Customer Item Option" ;
    rdfs:comment    "This represents a combination of a customer and an item." .

# Properties

sc:servableCustomer
    a            rdf:Property ;
    rdfs:label   "servable customer" ;
    rdfs:comment "Indicates a customer that you can served." .

sc:buyableSupplier
    a            rdf:Property ;
    rdfs:label   "buyable supplier" ;
    rdfs:comment "Indicates a supplier that you can buy from." .

sc:supportedItem
    a            rdf:Property ;
    rdfs:label   "supported item" ;
    rdfs:comment "Indicates an item that is supported for example by a specific location." .

sc:predictionModel
    a            rdf:Property ;
    rdfs:label   "prediction model" ;
    rdfs:comment "Indicates a prediction model." .

sc:replenishmentMethod
    a            rdf:Property ;
    rdfs:label   "replenishment method" ;
    rdfs:comment "Indicates how items are moved from one location to the other." .

sc:supplierItemOption
    a            rdf:Property ;
    rdfs:label   "supplier item option" ;
    rdfs:comment "Indicates the related supplier item option." .

sc:quantityRestrictions
    a            rdf:Property ;
    rdfs:label   "quantity restrictions" ;
    rdfs:comment "Indicates restrictions on the quantity of an item. The object ca be a schema:QuantitativeValue" .

sc:inventoryHoldingCosts
    a            rdf:Property ;
    rdfs:label   "inventory holding costs" ;
    rdfs:comment "Indicates the holding costs for an item." .

sc:leadTime
    a            rdf:Property ;
    rdfs:label   "lead time" ;
    rdfs:comment "Indicates the lead time of an item." .

sc:netOrderCost
    a            rdf:Property ;
    rdfs:label   "net order costs" ;
    rdfs:comment "Indicates the net costs of an order." .

sc:deliveredQuantity
    a            rdf:Property ;
    rdfs:label   "delivered quantity" ;
    rdfs:comment "Indicates the delivered quantity of an ordered item." .

sc:supplier
    a            rdf:Property ;
    rdfs:label   "supplier" ;
    rdfs:comment "Indicates the supplier of a SupplierItemLeadTimeOption." .

